Good advancements

RAlist/test.fst
@@ -1,9 +1,30 @@
 module Test
 
+
 open FStar.List.Tot.Base
+open FStar.Mul
+open FStar.Tactics
+
+(* Some util functions I couldnt find
+*)
+
+val pow : a:pos -> e:nat -> pos
+let rec pow a e = match e with
+    | 0 -> 1
+    | x -> a * (pow a (x - 1))
+
+val pow_distr_sums_on_e : e1:nat -> e2:nat -> a:pos -> Lemma (pow a (e1 + e2) = (pow a e1)*(pow a e2))
+let rec pow_distr_sums_on_e e1 e2 a = match e2 with
+  | 0 -> ()
+  | x -> pow_distr_sums_on_e e1 (x - 1) a
+
+val pow_dec_on_e : e1:nat -> e2:nat{e2 > e1} -> a:pos -> Lemma (pow a e1 <= pow a e2)
+let pow_dec_on_e e1 e2 a = begin
+  pow_distr_sums_on_e (e2 - e1) e1 a
+end
 
 (*  comBiTree
-    comBitree is a COMplete BInary TREE with the height of the tree at type level
+    comBitree is a non empty COMplete BInary TREE with the height of the tree at type level
 *)
 type comBiTree 'a : (x:pos) -> Type =
     | Leaf : 'a -> comBiTree 'a 1
@@ -27,30 +48,108 @@ let rec preorder #x #b t = match t with
 
 (* Should I do a Lemma stating what preorder does? It'd look very similar to the implementation. *)
 
-val preorder_keeps_the_elements : #n:pos -> t:comBiTree 'a n -> Lemma (length (preorder t) = treeSize t)
+val append_len: l1:list 'a -> l2:list 'a
+                -> Lemma (requires True)
+                        (ensures (length ( l1 @ l2) = length l1 + length l2))
+let rec append_len l1 l2 = match l1 with
+    | [] -> ()
+    | hd::tl -> append_len tl l2
 
+
+val random_lemma : 
+                 #b:Type -> 
+                 x:b -> 
+                 l1:list b -> 
+                 l2:list b -> 
+                 Lemma (length (x :: l1 @ l2) = 1 + length l1 + length l2)
+let rec random_lemma #b x l1 l2 = append_len (x::l1) l2
+
+val preorder_keeps_the_elements : #n:pos -> #b:Type -> t:comBiTree b n -> Lemma (length (preorder t) = treeSize t)
+let rec preorder_keeps_the_elements #n #b t = match t with
+    | Leaf _ -> ()
+    | Branch x t1 t2 -> begin
+      preorder_keeps_the_elements t1;
+      preorder_keeps_the_elements t2;
+      random_lemma x (preorder t1) (preorder t2)
+    end
+
+val preorder_has_the_root_first : 
+                                #n:pos -> 
+                                #b:eqtype ->
+                                x:b ->
+                                t1:comBiTree b n -> 
+                                t2:comBiTree b n -> 
+                                Lemma 
+                                  (preorder (Branch x t1 t2) = 
+                                    x :: ((preorder t1) @ (preorder t2)))
+let preorder_has_the_root_first #n #b x t1 t2 = () 
 
 (* raNode
    It's a non empty linked list of strictly increasing comBiTrees
+   With the height of the head tree at type level.
 *)
 type raNode 'a : (n:pos) -> Type =
     | Last : #m:pos -> comBiTree 'a m -> raNode 'a m
     | More : #m:pos -> #k:pos{k>m} -> comBiTree 'a m -> 
         raNode 'a k -> raNode 'a m
 
+val lenRan : #x:pos -> #b:Type -> r:raNode b x -> Tot (y:pos) (decreases r)
+let rec lenRan #x #b r  = match r with
+    | Last _ -> 1
+    | More _ m -> 1 + lenRan m
 
+val toList : #x:pos -> #b:Type -> r:raNode b x -> Tot (list b) (decreases r)
+let rec toList #x #b r = match r with
+    | Last t -> preorder t
+    | More t m -> preorder t @ (toList m)
 
-val sizeRan : #x:pos -> raNode 'a x -> y:pos{y = x}
-let sizeRan (r:raNode 'a 'n) = match r with
-    | Last t -> treeHeight t
-    | More t _ -> treeHeight t
-
+val sizeRan : #x:pos -> #b:Type -> r:raNode b x -> Tot (y:pos{y = length (toList r)}) (decreases r)
+let rec sizeRan #x #b r = match r with
+    | Last t -> (preorder_keeps_the_elements t; treeSize t)
+    | More t m -> begin
+      preorder_keeps_the_elements t;
+      append_len (preorder t) (toList m);
+      treeSize t + sizeRan m
+    end
 
 val headTree : #n:pos -> #b:Type -> raNode b n -> comBiTree b n 
 let headTree #n #b ran = match ran with
   | Last t -> t
   | More t _ -> t
 
+(*
+val ran_is_short_helper :
+                        #x:pos ->
+                        #x2:pos{x2 > x} ->
+                        #b:Type ->
+                        t:comBiTree b x ->
+                        r:raNode b x2 ->
+                        Lemma ( More t r
+*)
+(*
+val ran_is_short : 
+                  #x:pos ->
+                  #b:Type ->
+                  r:raNode b x ->
+                  Lemma (ensures sizeRan r + 1 > pow 2 (lenRan r + (x - 1))) (decreases r)
+let rec ran_is_short #x #b r = match r with
+  | Last t -> ()
+  | More t r2 -> let k = treeHeight (headTree r2) in
+  begin
+    ran_is_short r2;
+    pow_distr_sums_on_e (lenRan r) (x - 1) 2;
+    pow_distr_sums_on_e (lenRan r2) (k - 1) 2
+  end
+*)
+(*
+starting at 1
+1 4 11 26
+2 4 8  16
+
+starting at 3
+7 22 53
+8
+*)
 
 (* ralist
    It's a Random Access list, it can be:
@@ -61,18 +160,20 @@ let headTree #n #b ran = match ran with
 type ralist 'a = 
     | Empty : ralist 'a
     | Once : #n:pos -> raNode 'a n -> ralist 'a
-    | Twice : #n:pos -> comBiTree 'a n -> 
-        raNode 'a n -> ralist 'a
+    | Twice : #n:pos -> comBiTree 'a n -> raNode 'a n -> ralist 'a
         
 let empty = Empty
 
-
-//val insertTreeInNode : #a:Type -> #x:nat{x>0} -> #y:nat{y>0} -> comBiTree a x -> raNode a y -> #z:nat -> ralist a z
+val raToList : #b:Type -> ralist b -> list b
+let raToList #b ra = match ra with
+    | Empty -> []
+    | Once ran -> toList ran
+    | Twice t r -> preorder t @ toList r
 
 val insert : #b:Type -> b -> ralist b -> ralist b
 let insert #b a ral = match ral with
     | Empty -> Once (Last (Leaf a))
-    | Once ran -> let sRan = sizeRan ran in
+    | Once ran -> let sRan = treeHeight (headTree ran) in
     	if (1 < sRan) 
     	then Once (More (Leaf a) ran)
         else Twice (Leaf a) ran
@@ -81,10 +182,53 @@ let insert #b a ral = match ral with
         match ran2 with 
     	  | Last t2 -> Once (Last (Branch a t t2))
           | More t2 ran3 -> let newTree = Branch a t t2 in
-                 if (sizeRan ran3) > (treeHeight newTree)
+                 if (treeHeight (headTree ran3)) > (treeHeight newTree)
                  then Once (More newTree ran3)
                  else Twice newTree ran3
       end
+
+val helper_lemma : #b:eqtype -> x:b -> l1:list b -> l2:list b -> Lemma ((x::l1) @ l2 = x::(l1@l2))
+let rec helper_lemma #b x l1 l2 = ()
+
+val other_helper_lemma : #b:eqtype -> l1:list b -> l2:list b -> l3:list b -> Lemma ((l1@l2)@l3 = l1@(l2@l3))
+let rec other_helper_lemma #b l1 l2 l3 = match l1 with
+  | [] -> ()
+  | hd::tl -> (helper_lemma hd tl l2; helper_lemma hd (tl@l2) l3; other_helper_lemma tl l2 l3)
+
+val helper_fun : #b:Type -> ralist b -> bool
+let helper_fun #b r = match r with
+  | Empty -> true 
+  | _ -> false
+  
+val insert_lemma : 
+                 #b:eqtype -> 
+                 x:b -> 
+                 rl:ralist b -> 
+                 Lemma (raToList (insert x rl) = x :: (raToList rl))
+let insert_lemma #b x rl = match rl with
+  | Empty -> ()
+  | Once ran -> begin 
+    match treeHeight (headTree ran) with
+      | 1 -> ()
+      | _ -> ()
+  end
+  | Twice t ran2 -> begin
+    match ran2 with 
+      | Last t2 -> preorder_has_the_root_first x t t2
+      | More t2 ran -> let newTree = Branch x t t2 in
+        if (treeHeight (headTree ran)) > (treeHeight newTree)
+        then (
+          preorder_has_the_root_first x t t2;
+          helper_lemma x (preorder t @ preorder t2) (toList ran);
+          other_helper_lemma (preorder t) (preorder t2) (toList ran)
+        )
+        else (
+          preorder_has_the_root_first x t t2; 
+          helper_lemma x (preorder t @ preorder t2) (toList ran);
+          other_helper_lemma (preorder t) (preorder t2) (toList ran)
+        )
+  end
+
 
 val lenNode : #b:Type -> #n:nat{n > 0} -> rs:raNode b n -> Tot (x:nat{x >= pow2 n - 1}) (decreases rs)
 let rec lenNode #b #n ran = match ran with
@@ -96,6 +240,7 @@ let len #b ral = match ral with
   | Empty -> 0
   | Once ran -> lenNode ran
   | Twice t ran -> pow2 (treeHeight t) - 1 + lenNode ran
+
 
 val head : #b:Type -> l:ralist b{len l > 0} -> b
 let head #b ral = match ral with
@@ -114,6 +259,10 @@ let head #b ral = match ral with
       | Branch a _ _ -> a
       end
 
+val head_lemma : #b:eqtype -> x:b -> rl:ralist b{len rl > 0} -> Lemma (head (insert x rl) = x)
+let head_lemma #b x rl = insert_lemma x rl
+
+
 val tail : #b:Type -> #n:pos -> l:ralist b{len l = n} -> m:ralist b{len m = n - 1}
 let tail #b #n ral = match ral with
   | Once ran -> begin match ran with
@@ -130,6 +279,9 @@ let tail #b #n ral = match ral with
       | Leaf a -> Once nxtRan
       | Branch _ t1 t2 -> Twice t1 (More t2 nxtRan)
     end
+
+//val tail_lemma : #b:Type -> x:b -> rl:ralist b -> Lemma (tail (insert x rl) = rl)
+//let
 
 // fuel < 3*log2(i)
 val lookupTree : #b:Type -> #m:pos -> i:nat{i < pow2 m - 1}  -> #fuel:pos{fuel = m}(*Here I'd like to state that fuel == log2(i), it's stronger*) -> comBiTree b m -> b
